
# Calculus II


Today's Topics:
 The Indefinite Integral: The Antiderivative;
 Common Rules of Integration;
 The Definite Integral: The Area under the Curve;
 Integration by Substitution;
 Integration by Parts
 
Much of the material and examples for this lecture are taken from Simon \& Blume (1994) \emph{Mathematics for Economists} and from Boyce \& Diprima (1988) \emph{Calculus}



## The Indefinite Integral: The Antiderivative

So far, we've been interested in finding the derivative $g=f'$ of a function $f$.  However, sometimes we're interested in exactly the reverse:  finding the function $f$ for which $g$ is its derivative.  We refer to $f$ as the {\bf antiderivative} of $g$.

Let $DF$ be the derivative of $F$.  And let $DF(x)$ be the derivative of $F$ evaluated at $x$.  Then the antiderivative is denoted by $D^{-1}$ (i.e., the inverse derivative).  If $DF=f$, then $F=D^{-1}f$.

__Indefinite Integral__:  Equivalently, if $F$ is the antiderivative of $f$, then $F$ is also called the indefinite integral of $f$ and written $F(x)=\int\limits f(x)dx$.

\begin{framed}
Examples:
	\parbox[c]{3.75in}{
	\begin{enumerate}
		\item $\int\limits \frac{1}{x^2}dx=$
		\item $\int\limits 3e^{3x}dx=$
		\item $\int\limits (x^2-4) dx=$
	\end{enumerate}}
\begin{comment}
\parbox[c]{1in}{\,  {\includegraphics[width=1in, angle = 270]{derinteg.eps}}}
\end{comment}
\end{framed}
	
Notice from these examples that while there is only a single derivative for any function, there are multiple antiderivatives: one for any arbitrary constant $c$.  $c$ just shifts the curve up or down on the $y$-axis.  If more info is present about the antiderivative --- e.g., that it passes through a particular point --- then we can solve for a specific value of $c$.
\end{itemize}

## Common Rules of Integration

\begin{itemize}
\item $\int a f(x)dx = a\int f(x)dx$
\item $\int [f(x)+g(x)]dx=\int f(x)dx + \int g(x)dx$
\item $\int x^n dx = \frac{1}{n+1} x^{n+1} + c $
\item $\int e^x dx = e^x +c$
\item $\int \frac{1}{x} dx = \ln x + c$
\item $\int e^{f(x)}f'(x)dx = e^{f(x)}+c$
\item $\int [f(x)]^n f'(x)dx = \frac{1}{n+1}[f(x)]^{n+1}+c$
\item $\int \frac{f'(x)}{f(x)}dx=\ln f(x) + c$
\end{itemize}

\begin{framed}
Examples:
\begin{enumerate}
	\item $\int 3x^2 dx= $
	\item $\int (2x+1)dx=$
	\item $\int e^x e^{e^x} dx = $
\end{enumerate}
\end{framed}




## The Definite Integral: The Area under the Curve

__Riemann Sum__:  Suppose we want to determine the area $A(R)$ of a region $R$ defined by a curve $f(x)$ and some interval $a\le x \le b$.  One way to calculate the area would be to divide the interval $a\le x\le b$ into $n$ subintervals of length $\Delta x$ and then approximate the region with a series of rectangles, where the base of each rectangle is $\Delta x$ and the height is $f(x)$ at the midpoint of that interval.  $A(R)$ would then be approximated by the area of the union of the rectangles, which is given by $$S(f,\Delta x)=\sum\limits_{i=1}^n f(x_i)\Delta x$$ and is called a Riemann sum.

As we decrease the size of the subintervals $\Delta x$, making the rectangles "thinner," we would expect our approximation of the area of the region to become closer to the true area.  This gives the limiting process $$A(R)=\lim\limits_{\Delta x\to 0}\sum\limits_{i=1}^n f(x_i)\Delta x$$

__Riemann Integral__:  If for a given function $f$ the Riemann sum approaches a limit as $\Delta x \to 0$, then that limit is called the Riemann integral of $f$ from $a$ to $b$.  Formally, $$\int\limits_a^b f(x) dx= \lim\limits_{\Delta x\to 0} \sum\limits_{i=1}^n f(x_i)\Delta x$$

__Definite Integral__: We use the notation $\int\limits_a^b f(x) dx$ to denote the definite integral of $f$ from $a$ to $b$.  In words, the definite integral $\int\limits_a^b f(x)dx$ is the area under the ``curve" f(x) from $x=a$ to $x=b$.

__First Fundamental Theorem of Calculus__:  Let the function $f$ be bounded on $[a,b]$ and continuous on $(a,b)$.  Then the function $$F(x)=\int\limits_a^x f(t)dt, \quad a\le x\le b$$ has a derivative at each point in $(a,b)$ and $$F'(x)=f(x), \quad a<x<b$$  This last point shows that differentiation is the inverse of integration.

__Second Fundamental Theorem of Calculus__:  Let the function $f$ be bounded on $[a,b]$ and continuous on $(a,b)$.  Let $F$ be any function that is continuous on $[a,b]$ such that $F'(x)=f(x)$ on $(a,b)$.  Then $$\int\limits_a^bf(x)dx = F(b)-F(a)$$

\textbf{Procedure to calculate a ``simple" definite integral} $\int\limits_a^b f(x)dx$:

1. Find the indefinite integral $F(x)$.
2. Evaluate $F(b)-F(a)$.

\begin{framed}
Examples:
\begin{enumerate}
		\item $\int\limits_1^3 3x^2 dx=  $
		\item $\int\limits_{-2}^2 e^x e^{e^x} dx =$
\end{enumerate}
\end{framed}

Properties of Definite Integrals:
\begin{enumerate}
		\item \parbox[t]{2in}{$\int\limits_a^a f(x)dx=0$}\parbox[t]{4in}{There is no area below a point.}
		\item \parbox[t]{2in}{$\int\limits_a^b f(x)dx=-\int\limits_b^a f(x)dx$}\parbox[t]{4in}{Reversing the limits changes the sign of the integral.}
		\item $\int\limits_a^b [\alpha f(x)+\beta g(x)]dx = \alpha \int\limits_a^b f(x)dx + \beta \int\limits_a^b g(x)dx$
		\item $\int\limits_a^b f(x) dx +\int\limits_b^c f(x)dx = \int\limits_a^c f(x)dx$
\end{enumerate}

\begin{framed}
Examples:
\begin{enumerate}
		\item $\int\limits_1^1 3x^2 dx = $ 
		\item $\int\limits_0^4 (2x+1)dx= $ 
		\item $\int\limits_{-2}^0 e^x e^{e^x} dx + \int\limits_0^2 e^x e^{e^x} dx =$
	\end{enumerate}
\end{framed}




## Integration by Substitution

Sometimes the integrand doesn't appear integrable using common rules and antiderivatives.  A method one might try is __integration by substitution__, which is related to the Chain Rule.

Suppose we want to find the indefinite integral $\int g(x)dx$ and assume we can identify a function $u(x)$ such that $g(x)=f[u(x)]u'(x)$. Let's refer to the antiderivative of $f$ as $F$.  Then the chain rule tells us that $\frac{d}{dx} F[u(x)]=f[u(x)]u'(x)$.  So, $F[u(x)]$ is the antiderivative of $g$.  We can then write $$\int g(x) dx= \int f[u(x)]u'(x)dx = \int \frac{d}{dx} F[u(x)]dx = F[u(x)]+c$$

__Procedure to determine the indefinite integral $\int g(x)dx$ by the method of substitution:__

1. Identify some part of $g(x)$ that might be simplified by substituting in a single variable $u$ (which will then be a function of $x$).
2. Determine if $g(x)dx$ can be reformulated in terms of $u$ and $du$.
3. Solve the indefinite integral.
4. Substitute back in for $x$


Substitution can also be used to calculate a definite integral. Using the same procedure as above, \[\int\limits_a^b g(x)dx=\int\limits_c^d f(u)du = F(d)-F(c)\]
where $c=u(a)$ and $d=u(b)$.

Example: $\int x^2 \sqrt{x+1}dx$

\vspace{6pt}

The problem here is the $\sqrt{x+1}$ term.  However, if the integrand had $\sqrt{x}$ times some polynomial, then we'd be in business.  Let's try $u=x+1$.  Then $x=u-1$ and $dx=du$. Substituting these into the above equation, we get 

\begin{eqnarray}
			\int x^2\sqrt{x+1}dx&=&\int (u-1)^2\sqrt{u}du\nonumber\\
			&=&\int (u^2-2u+1)u^{1/2}du\nonumber\\
			&=&\int (u^{5/2}-2u^{3/2}+u^{1/2})du\nonumber
\end{eqnarray}

We can easily integrate this, since it's just a polynomial.  Doing so and substituting $u=x+1$ back in, we get \[\int x^2\sqrt{x+1}dx=2(x+1)^{3/2}\left[\frac{1}{7}(x+1)^2 -
\frac{2}{5}(x+1)+\frac{1}{3}\right]+c\]

For the above problem, we could have also used the substitution $u=\sqrt{x+1}$.  Then $x=u^2-1$ and $dx=2u du$.  Substituting these in, we get $$\int x^2\sqrt{x+1}dx=\int (u^2-1)^2 u 2u du$$ which when expanded is again a polynomial and gives the same result as above.

Another Example $\int\limits_0^1 \frac{5e^{2x}}{(1+e^{2x})^{1/3}}dx$

\vspace{6pt}

When an expression is raised to a power, it's often helpful to use this expression as the basis for a substitution.  So, let $u=1+e^{2x}$. Then $du=2e^{2x}dx$ and we can set $5e^{2x}dx=5du/2$.    Additionally, $u=2$ when $x=0$ and $u=1+e^2$ when $x=1$.  Substituting all of this in, we get
\begin{eqnarray}
			\int\limits_0^1 \frac{5e^{2x}}{(1+e^{2x})^{1/3}}dx
			&=& \frac{5}{2}\int\limits_2^{1+e^2}\frac{du}{u^{1/3}}\nonumber\\
			&=& \frac{5}{2}\int\limits_2^{1+e^2} u^{-1/3}du\nonumber\\
			&=& \left. \frac{15}{4} u^{2/3} \right|_2^{1+e^2}\nonumber\\
			&=& 9.53\nonumber
\end{eqnarray}



## Integration by Parts, or Ultraviolet Voodoo


Another useful integration technique is {\bf integration by parts}, which is related to the Product Rule of differentiation. The product rule states that $$\frac{d}{dx}(uv)=u\frac{dv}{dx}+v\frac{du}{dx}$$  Integrating this and rearranging, we get $$\int u\frac{dv}{dx}dx= u v - \int v \frac{du}{dx}dx$$ or $$\int u(x) v'(x)dx=u(x)v(x) - \int v(x)u'(x)dx$$
More frequently remembered as $$\int u dv = u v - \int v du$$ where $du=u'(x)dx$ and $dv=v'(x)dx$.


For definite integrals: $\int\limits_a^b u\frac{dv}{dx}dx = \left. u v \right|_a^b - \int\limits_a^b v \frac{du}{dx}dx$

Our goal here is to find expressions for $u$ and $dv$ that, when substituted into the above equation, yield an expression that's more easily evaluated.
	
Examples:

\begin{framed}
\begin{enumerate}
		\item $\int x e^{ax} dx$
		\item $\int x^n e^{ax} dx$\\
		\item $\int x^3 e^{-x^2} dx$\\
\vspace{10pt}
\end{enumerate}
\end{framed}